refactor: drop variable bound index from Program
Let's try an even less dependently typed approach

EffectSSA/Rewrites/Basic.lean
@@ -16,18 +16,16 @@ namespace EffectSSA
 A program fragment is simply a program with some designated return variables
 at the end of said program.
 -/
-@[grind]
-structure ProgramFragment τ n where
-  program : Program τ n
-  returnVars : List (Var program.results)
+structure ProgramFragment τ where
+  program : Program τ
+  returnVars : List Var
 
 /--
 A rewrite consists of two program fragments.
 -/
-@[grind]
-structure Rewrite τ n where
-  src : ProgramFragment τ n
-  tgt : ProgramFragment τ n
+structure Rewrite τ where
+  src : ProgramFragment τ
+  tgt : ProgramFragment τ
 
 /-!
 ## Structural Lemmas
@@ -42,20 +40,17 @@ theorem ProgramFragment.program_mk : (mk p vs).program = p := rfl
 --------------------------------------------------------------------------------
 -/
 
-@[simp, grind =]
-def ProgramFragment.externalResults (p : ProgramFragment τ n) : Nat := p.returnVars.length
-
 /--
 A program fragment is welltyped, for a given set of return types, when
 (a) the program is welltyped, producing an output context `Δ`, and
 (b) each return variable is assigned the expected return type in `Δ`.
 -/
 @[grind =]
-def ProgramFragment.WellTyped (Γ : Context τ n) (p : ProgramFragment τ n)
+def ProgramFragment.WellTyped (Γ : Context τ) (p : ProgramFragment τ)
     (returnTypes : List τ.Typ) : Prop :=
-  ∃ (m : _) (Δ : Context τ m),
+  ∃ (Δ : Context τ),
     Program.WellTypedWith Γ p.program Δ ∧ Δ.isUnrestricted
-    ∧ (∀ (i : Fin p.externalResults), Δ[p.returnVars[i].toNat]? = returnTypes[i]?)
+    ∧ (∀ (i : Fin p.returnVars.length), Δ[p.returnVars[i]]? = returnTypes[i]?)
 
 open ProgramFragment (WellTyped) in
 /--
@@ -63,23 +58,18 @@ A rewrite is wellformed, if both fragments are welltyped, under the same context
 and with the same expected return types.
 -/
 @[grind =]
-def Rewrite.WellFormed (Γ : Context τ n) (r : Rewrite τ n) : Prop :=
+def Rewrite.WellFormed (Γ : Context τ) (r : Rewrite τ) : Prop :=
   ∃ ts, WellTyped Γ r.src ts ∧ WellTyped Γ r.tgt ts
 
 /-! ### Welltypedness of a `ProgramFragment` is decidable -/
-instance (p : ProgramFragment τ n) : Decidable (p.WellTyped Γ ts) :=
+instance (p : ProgramFragment τ) : Decidable (p.WellTyped Γ ts) :=
   match p.program.typeCheck Γ with
   | .isFalse h => .isFalse <| by grind
-  | .isTrue (m:=m) Δ h₁ h₂ hm =>
-      if h : ∀ (i : Fin p.externalResults), Δ[p.returnVars[i].toNat]? = ts[i]? then
+  | .isTrue Δ h₁ h₂ =>
+      if h : ∀ (i : Fin p.returnVars.length), Δ[p.returnVars[i]]? = ts[i]? then
         .isTrue (by grind)
       else
-        .isFalse <| by
-          simp only [ProgramFragment.WellTyped, ProgramFragment.externalResults, Fin.getElem_fin,
-            Fin.getElem?_fin, not_exists, not_and, not_forall]
-          intro m Δ' h'
-          rcases Program.WellTyped.unique h' h₁ with ⟨rfl, rfl⟩
-          grind
+        .isFalse (by grind)
 
 /-!
 ## Semantics Correctness Constraints
@@ -92,17 +82,17 @@ open Semantics in
 Execute all instructions in a program fragment sequentially,
 but return only the values computed for the designated return variables.
 -/
-def ProgramFragment.exec (env : Environment τ n) (p : ProgramFragment τ n) :
+def ProgramFragment.exec (env : Environment τ) (p : ProgramFragment τ) :
     ExecM τ (List τ.Val) := do
   let env ← p.program.exec env
-  return p.returnVars.map env.get
+  p.returnVars.mapM env.get
 
 /--
 A rewrite is correct, if the source and target fragments compute the same values
 for the return variables (given the same environment).
 -/
-def Rewrite.Correct (r : Rewrite τ n) : Prop :=
+def Rewrite.Correct (r : Rewrite τ) : Prop :=
   -- FIXME: this is actually too granular, as it looks for strict equality of
   --        of traces, whereas we want to consider something a bit looser, e.g.
   --        to disregard the specific order of load events.
-  ∀ env, r.src.exec env = r.tgt.exec env
+  ∀ {env} {Γ}, env.WellTyped Γ → r.src.exec env = r.tgt.exec env
