EffectSSA/Semantics/Environment.lean
@@ -34,8 +34,8 @@ inductive Ty.TVal : τ.Typ → Type where
 def Ty.Val : Type := Σ t, τ.TVal t
 -- FIXME: maybe `Ty.Val` ought to be a structure? We'll evaluate later.
 
-structure Semantics.Environment τ [MemoryModel τ] (n : Nat) where
-  ofVector :: toVec : List.Vector τ.Val n
+structure Semantics.Environment τ [MemoryModel τ] where
+  ofList :: toList : List τ.Val
 
 /-!
 ## Definitions
@@ -70,19 +70,27 @@ namespace Semantics.Environment
 /-! #### Environment Getters -/
 
 /--
-`env.get v` retrieves the (untyped) value environment `env` associates with
-the variable `v`.
+`env.get? v` retrieves the (untyped) value environment `env` associates with
+the variable `v`. Returns `none` if the variable does not exist.
 -/
-def get (env : Environment τ n) (v : Var n) : τ.Val :=
-  env.toVec[v.toFin]
+def get? (env : Environment τ) (v : Var) : Option τ.Val :=
+  env.toList[v.toNat]?
+
+/--
+`env.get v` retrieves the (untyped) value environment `env` associates with
+the variable `v`. Throws a TypErr if the variable does not exist.
+-/
+def get (env : Environment τ) (v : Var) : ExecM τ τ.Val :=
+  StateT.lift (env.get? v)
 
 /--
 `env.getAs? v t` retrieves the value environment `env` associates with the
 variable `v`, and then attempts to coerce this to be a typed value of type `t`.
-Returns `none` if `v` has a type different from `t`.
+Returns `none` if `v` has a type different from `t`, or if `v` is not present in
+the environment.
 -/
-def getAs? (env : Environment τ n) (v : Var n) (t : τ.Typ) : Option (τ.TVal t) :=
-  let val := env.get v
+def getAs? (env : Environment τ) (v : Var) (t : τ.Typ) : Option (τ.TVal t) := do
+  let val ← env.get? v
   if h : val.1 = t then
     some <| h ▸ val.2
   else
@@ -91,21 +99,22 @@ def getAs? (env : Environment τ n) (v : Var n) (t : τ.Typ) : Option (τ.TVal t
 /--
 `env.getAs v t` retrieves the value environment `env` associates with a
 variable `v`, and then attempts to coerce this to be a typed value of type `t`.
-Throws a type error if `v` has a type different from `t`.
+Throws a type error if `v` has a type different from `t`, or if `v` is not
+present in the environment.
 
 See also `Environment.getAs?`, which returns none instead.
 -/
-def getAs (env : Environment τ n) (v : Var n) (t : τ.Typ) : ExecM τ (τ.TVal t) :=
+def getAs (env : Environment τ) (v : Var) (t : τ.Typ) : ExecM τ (τ.TVal t) :=
   StateT.lift (env.getAs? v t)
 
 /-- Retrieve a pointer via `getAs`. -/
-def getPtr (env : Environment τ n) (v : Var n) : ExecM τ τ.Ptr := env.getAs v .ptr
+def getPtr (env : Environment τ) (v : Var) : ExecM τ τ.Ptr := env.getAs v .ptr
 
 /-- Retrieve an effect trace via `getAs`. -/
-def getEff (env : Environment τ n) (v : Var n) : ExecM τ (Trace τ) := env.getAs v .eff
+def getEff (env : Environment τ) (v : Var) : ExecM τ (Trace τ) := env.getAs v .eff
 
 /-- Retrieve a data value via `getAs`. -/
-def getData (env : Environment τ n) (v : Var n) (t : τ.DType) : ExecM τ (τ.DVal t) :=
+def getData (env : Environment τ) (v : Var) (t : τ.DType) : ExecM τ (τ.DVal t) :=
   env.getAs v (.data t)
 
 /-! #### Environment Constructors -/
@@ -113,13 +122,25 @@ def getData (env : Environment τ n) (v : Var n) (t : τ.DType) : ExecM τ (τ.D
 /--
 `env.snoc x` adds a new variable to environment `env` assigning value `x` to it.
 -/
-def snoc (x : τ.Val) (env : Environment τ n) : Environment τ (n + 1) :=
-  ⟨env.toVec.cons x⟩
+def snoc (x : τ.Val) (env : Environment τ) : Environment τ :=
+  ⟨env.toList.cons x⟩
 
 /-! #### Environment Modification -/
 
 /--
 `env.eraseVar v` removes a variable `v` from an environment `env`.
 -/
-def eraseVar (env : Environment τ n) (v : Var n) : Environment τ (n - 1) :=
-  ⟨env.toVec.eraseIdx v.toFin⟩
+def eraseVar (env : Environment τ) (v : Var) : Environment τ :=
+  ⟨env.toList.eraseIdx v.toNat⟩
+
+end Semantics.Environment
+
+
+/-!
+## WellTyped
+--------------------------------------------------------------------------------
+-/
+namespace Semantics.Environment
+
+def WellTyped (Γ : Context τ) (env : Environment τ) : Prop :=
+  ∀ (v : Var) (t : τ.Typ), Γ[v]? = some t ↔ (env.getAs? v t).isSome
