EffectSSA/Syntax/Basic.lean
@@ -20,32 +20,95 @@ namespace EffectSSA
 /--
 `Instruction τ` represents a single instruction (including arguments).
 -/
-inductive Instruction (τ : Ty) (n : Nat) where
+inductive Instruction (τ : Ty) where
   -- Basic memory ops with implicit effects
-  | loadI (t : τ.DType) (p : Var n)
-  | storeI (t : τ.DType) (p : Var n) (x : Var n)
-  | allocI (t : τ.DType) (p : Var n)
-  | freeI (t : τ.DType) (p : Var n)
+  | loadI (t : τ.DType) (p : Var)
+  | storeI (t : τ.DType) (p : Var) (x : Var)
+  | allocI (t : τ.DType) (p : Var)
+  | freeI (t : τ.DType) (p : Var)
   -- Basic memory ops in EffectSSA form
-  | loadE (t : τ.DType) (eff : Var n) (p : Var n)
-  | storeE (t : τ.DType) (eff : Var n) (p : Var n) (x : Var n)
-  | allocE (t : τ.DType) (eff : Var n) (p : Var n)
-  | freeE (t : τ.DType) (eff : Var n) (p : Var n)
+  | loadE (t : τ.DType) (eff : Var) (p : Var)
+  | storeE (t : τ.DType) (eff : Var) (p : Var) (x : Var)
+  | allocE (t : τ.DType) (eff : Var) (p : Var)
+  | freeE (t : τ.DType) (eff : Var) (p : Var)
   -- FIXME: the draft also has stack address & constant value instruction
   -- Effect Bookkeeping
-  | split (eff : Var n)
-  | merge (eff₁ : Var n) (eff₂ : Var n)
+  | split (eff : Var)
+  | merge (eff₁ : Var) (eff₂ : Var)
   | createEff
-  | consumeEff (e : Var n)
+  | consumeEff (e : Var)
 
 /--
-`i.results` gives the number of (live) free variables available after executing
-an instruction `i`, taking into account free variables available to `i`.
+A program is a (possibly empty) sequence of instructions.
+It is thus morally similar to a `List (Instruction ..)`, except that `Program`
+additionally tracks the bound on free variables available to each instruction.
+
+Programs grow upwards, such that `cons i p` represents `i ; p`,
+first executing instruction `i` and then the rest of the program `p`.
+-/
+inductive Program (τ : Ty) : Type where
+  | nil : Program τ
+  | cons : Instruction τ → Program τ → Program τ
+  -- toList : List (Instruction τ)
+
+/-
+FIXME: I wonder if I'm not getting the worst of both worlds by doing intrinsically
+tracked de Bruijn indices but extrinsically typed. To track the indices, `Program`
+has become a custom inductive, instead of just a `List`, so I'm going to have to
+implement a bunch of API for it anyway.
+-/
+
+/-!
+## Definitions
+--------------------------------------------------------------------------------
+-/
+section Defs
+namespace Program
+
+/-! ### Pseudo-constructors -/
+/--
+`i ;> p` is the preferred spelling for adding an instruction to the
+front of a program.
+-/
+infixl:67 " ;> " => Program.cons
+
+def toList : Program τ → List (Instruction τ)
+  | .nil => []
+  | i ;> p => i :: p.toList
+
+def ofList : List (Instruction τ) → Program τ
+  | [] => .nil
+  | i :: p => i ;> ofList p
+
+-- @[match_pattern]
+-- def Program.nil : Program τ := Program.mk []
+-- @[match_pattern]
+-- def Program.cons (i : Instruction τ) (p : Program τ) : Program τ :=
+--   Program.mk (i :: p.toList)
+
+/-! ### Folds -/
+
+@[inherit_doc List.foldl]
+def foldl (f : α → Instruction τ → α) (init : α) (p : Program τ) :=
+  p.toList.foldl f init
+
+@[inherit_doc List.foldlM]
+def foldlM [Monad m] (f : α → Instruction τ → m α) (init : α) (p : Program τ) :=
+  p.toList.foldlM f init
+
+end Program
+
+
+/-! ### Resulting variables -/
+
+/--
+`i.results n` gives the number of (live) free variables available after executing
+an instruction `i`, assuming `i` has access to `n` free variables.
 
 Here, live means that any linear variables consumed by `i` are excluded.
 -/
 @[grind =]
-def Instruction.results : Instruction τ n → Nat
+def Instruction.results (n : Nat) : Instruction τ → Nat
   | loadI .. => n + 1
   | storeI .. => n
   | allocI .. => n
@@ -60,53 +123,19 @@ def Instruction.results : Instruction τ n → Nat
   | consumeEff .. => n - 1
 
 /--
-A program is a (possibly empty) sequence of instructions.
-It is thus morally similar to a `List (Instruction ..)`, except that `Program`
-additionally tracks the bound on free variables available to each instruction.
-
-Programs grow upwards, such that `cons i p` represents `i ; p`,
-first executing instruction `i` and then the rest of the program `p`.
--/
-inductive Program (τ : Ty) : Nat → Type where
-  | nil : Program τ n
-  | cons : (i : Instruction τ n) → Program τ i.results → Program τ n
-
-/-
-FIXME: I wonder if I'm not getting the worst of both worlds by doing intrinsically
-tracked de Bruijn indices but extrinsically typed. To track the indices, `Program`
-has become a custom inductive, instead of just a `List`, so I'm going to have to
-implement a bunch of API for it anyway.
--/
-
-/-!
-## Definitions
---------------------------------------------------------------------------------
--/
-section Defs
-
-/--
-`p.results` gives the number of *live* free variables available after executing
-program `p`.
+`p.results n` gives the number of *live* free variables available after executing
+program `p`, assuming `p` has access to `n` free variables.
 
 Here, live means that any linear variables that have already been
 consumed during the execution of `p` are explicitly excluded.
 -/
-def Program.results : Program τ n → Nat
-  | nil => n
-  | cons _ p => results p
+def Program.results (n : Nat) (p : Program τ) : Nat :=
+  p.foldl Instruction.results n
 
 /--
-`i ;> p` is the preferred spelling for adding an instruction to the
-front of a program.
+`p ++ q` concatenates two programs.
 -/
-infixl:67 " ;> " => Program.cons
-
-/--
-`p.append q` concatenates two programs.
-
-NOTE: we cannot use standard `++` notation for this, as the type of `q`
-depends on `p`.
--/
-def Program.append : (p : Program τ n) → Program τ p.results → Program τ n
-  | .nil, q => q
+def Program.append : Program τ → Program τ → Program τ
+  | nil, q => q
   | i ;> p, q => i ;> (p.append q)
+instance : Append (Program τ) where append := Program.append
