EffectSSA/Syntax/Var.lean
@@ -4,7 +4,7 @@ import Qq
 /-!
 # Variables
 
-This file defines `Var n`, the type of program variables with an upper bound.
+This file defines `Var`, the type of program variables with an upper bound.
 
 -/
 namespace EffectSSA
@@ -15,10 +15,10 @@ namespace EffectSSA
 -/
 
 /--
-`Var n` is a de Bruijn index representing a variable, given an upper bound `n`
+`Var` is a de Bruijn index representing a variable, given an upper bound `n`
 on the number of available variables.
 -/
-def Var n := Fin n
+def Var := Nat
 
 /-!
 ## Definitions
@@ -27,20 +27,11 @@ def Var n := Fin n
 namespace Var
 
 /-- Return the underlying index of a variable. -/
-def toFin (v : Var n) : Fin n := v
+def toNat (v : Var) : Nat := v
 /-- Construct a variable from its index. -/
-def ofFin (i : Fin n) : Var n := i
-/-- Return the underlying index of a variable. -/
-def toNat (v : Var n) : Nat := v.toFin.val
+def ofNat (i : Nat) : Var := i
 
-/-- The bound on a variable `Var n` may implicitly be weakened to `n + 1`. -/
-instance : Coe (Var n) (Var <| n + 1) where coe := Fin.succ
-
-/--
-A placeholder variable, used for prototyping when we don't care about the
-specific variable index.
--/
-def placeholder {n : Nat} : Var (n + 1) := (0 : Fin _)
+def succ (v : Var) : Var := ofNat (v.toNat + 1)
 
 /-!
 ### Metaprogramming API
@@ -48,11 +39,11 @@ def placeholder {n : Nat} : Var (n + 1) := (0 : Fin _)
 section Meta
 open Lean Qq
 
-instance : Lean.ToExpr (Var n) where
+instance : Lean.ToExpr Var where
   toExpr v :=
-    let i : Q(Fin $n) := toExpr v.toFin
-    q(Var.ofFin $i)
-  toTypeExpr := q(Var $n)
+    let i : Q(Nat) := toExpr v.toNat
+    q(Var.ofNat $i)
+  toTypeExpr := q(Var)
 
 end Meta
 
