EffectSSA/Semantics/Lemmas.lean
@@ -11,7 +11,7 @@ variable {τ} [MemoryModel τ]
 The following theorem does not quite work, because the `.results` are not
 nicely def-eq.
 -/
--- theorem Program.exec_append (p : Program τ n) (q : Program τ p.results) :
+-- theorem Program.exec_append (p : Program τ) (q : Program τ) :
 --     (p.append q).exec =
 --       have h := sorry
 --       fun env => (p.exec env >>= (q.cast h).exec) := by
