EffectSSA/Tests/Syntax/Notation.lean
@@ -21,33 +21,31 @@ At first, we have a few tests using `#check`, to have a baseline check for the
 parser in isolation from the printing code.
 -/
 
-/-- info: Program.nil : Program ?m.1 0 -/
+/-- info: Program.nil : Program ?m.1 -/
 #guard_msgs in #check program!()
-/-- info: Program.nil : Program ?m.1 0 -/
+/-- info: Program.nil : Program ?m.1 -/
 #guard_msgs in #check program!{}()
-/-- info: Program.nil : Program ?m.1 3 -/
+/-- info: Program.nil : Program ?m.1 -/
 #guard_msgs in #check program!{x, y, z}()
 
 -- set_option trace.EffectSSA true
 
 /--
-info: have this :=
-  Program.cons (Instruction.loadI u8 (Var.ofFin 0))
-    (Program.cons (Instruction.storeI u8 (Var.ofFin 1) (Var.ofFin 0)) Program.nil);
-this : Program TestTy 1
+info: have this := Instruction.loadI u8 (Var.ofNat 0) ;> (Instruction.storeI u8 (Var.ofNat 1) (Var.ofNat 0) ;> Program.nil);
+this : Program TestTy
 -/
 #guard_msgs in
-#check show Program TestTy _ from program!{p}(
+#check show Program TestTy from program!{p}(
   x := loadI[u8](p);
   storeI[u8](p, x)
 )
 
 /--
-info: have this := Program.cons (Instruction.split (Var.ofFin 0)) Program.nil;
-this : Program TestTy 1
+info: have this := Instruction.split (Var.ofNat 0) ;> Program.nil;
+this : Program TestTy
 -/
 #guard_msgs in
-#check show Program TestTy _ from program!{e}(
+#check show Program TestTy from program!{e}(
   e1, e2 := split(e)
 )
 
@@ -72,7 +70,7 @@ x_1 := loadI[EffectSSA.Tests.MyDType.u8](x_0)
 )
 -/
 #guard_msgs in
-#eval show Program TestTy _ from program!{p}(
+#eval show Program TestTy from program!{p}(
   x := loadI[u8](p);
   y := loadI[u8](p);
   storeI[u8](p, y)
@@ -81,12 +79,12 @@ x_1 := loadI[EffectSSA.Tests.MyDType.u8](x_0)
 
 /--
 info: program{x_0,x_1}(
-storeI[EffectSSA.Tests.MyDType.u8](x_1, x_0)
+storeI[EffectSSA.Tests.MyDType.u8](x_0, x_1)
   ⏎
 )
 -/
 #guard_msgs in
-#eval show Program TestTy 2 from program!{p, v}(
+#eval show Program TestTy from program!{p, v}(
   storeI[u8](p, v)
 )
 
@@ -98,33 +96,33 @@ allocI[EffectSSA.Tests.MyDType.u8](x_0)
 )
 -/
 #guard_msgs in
-#eval show Program TestTy 1 from program!{p}(
+#eval show Program TestTy from program!{p}(
   allocI[u8](p)
 )
 
 -- Test explicit side effect op
 /--
 info: program{x_0,x_1}(
-x_2,x_3 := loadE[EffectSSA.Tests.MyDType.u8](x_1, x_0)
+x_2,x_3 := loadE[EffectSSA.Tests.MyDType.u8](x_0, x_1)
   ⏎
 )
 -/
 #guard_msgs in
-#eval show Program TestTy 2 from program!{e, p}(
+#eval show Program TestTy from program!{e, p}(
   e', x := loadE[u8](e, p)
 )
 
 -- Test complex program
 /--
 info: program{x_0,x_1}(
-allocI[EffectSSA.Tests.MyDType.u8](x_1)
-  storeI[EffectSSA.Tests.MyDType.u8](x_1, x_0)
-  freeI[EffectSSA.Tests.MyDType.u8](x_1)
+allocI[EffectSSA.Tests.MyDType.u8](x_0)
+  storeI[EffectSSA.Tests.MyDType.u8](x_0, x_1)
+  freeI[EffectSSA.Tests.MyDType.u8](x_0)
   ⏎
 )
 -/
 #guard_msgs in
-#eval show Program TestTy _ from program!{p, x}(
+#eval show Program TestTy from program!{p, x}(
   allocI[u8](p);
   storeI[u8](p, x);
   freeI[u8](p)
@@ -139,7 +137,7 @@ x_0 := createEff
 )
 -/
 #guard_msgs in
-#eval show Program TestTy 0 from program!{}(
+#eval show Program TestTy from program!{}(
   e := createEff;
   consumeEff(e)
 )
