EffectSSA/Types/Lemmas.lean
@@ -6,19 +6,25 @@ import EffectSSA.Types.WellTyped
 namespace EffectSSA
 
 /-!
-## `grind` annotations
+## `grind` lemmas
 --------------------------------------------------------------------------------
 -/
 
 @[simp, grind =]
-theorem Program.wellTyped_nil_iff {Γ : Context τ n} {Δ : Context τ m} :
-    WellTypedWith Γ (.nil) Δ ↔ ∃ (h : n = m), h ▸ Γ = Δ := by
-  grind [Program.WellTypedWith]
+theorem Program.wellTyped_nil_iff {Γ Δ : Context τ} :
+    WellTypedWith Γ .nil Δ ↔ Γ = Δ := by
+  grind [WellTypedWith]
 
 @[simp, grind =]
-theorem Program.wellTyped_cons_iff (i : Instruction τ n) (p : Program τ i.results) :
+theorem Program.wellTyped_cons_iff (i : Instruction τ) (p : Program τ) :
     WellTypedWith Γ (i ;> p) Ξ ↔ (∃ Δ, i.WellTyped Γ Δ ∧ p.WellTypedWith Δ Ξ) := by
-  grind [Program.WellTypedWith]
+  grind [WellTypedWith]
+
+@[simp, grind =]
+theorem Program.WellTyped_nil_iff {Γ : Context τ} :
+    WellTyped Γ .nil ↔ Γ.isUnrestricted := by
+  simp [Program.WellTyped]
+
 
 open Instruction in attribute [grind ←]
   WellTyped.loadI
@@ -28,28 +34,79 @@ open Instruction in attribute [grind ←]
   WellTyped.createEff
   WellTyped.consumeEff
 
-open Program in attribute [grind →]
-  -- WellTypedWith.nil
-  WellTypedWith.cons
-
--- WellTypedWith ?_ (.nil) ?_
--- WellTypedWith ?_ (.cons ?_ ?_) ?_
 
 /-!
 ## Uniqueness of out contexts
 --------------------------------------------------------------------------------
 -/
 
+@[grind →]
 theorem Instruction.WellTyped.unique
-    {i : Instruction τ n} {Δ : Context τ m} {Δ' : Context τ m'}
+    {i : Instruction τ} {Δ Δ' : Context τ}
     (h₁ : i.WellTyped Γ Δ) (h₂ : i.WellTyped Γ Δ') :
-      ∃ (h : m = m'), Δ = h ▸ Δ' := by
-  grind
+      Δ = Δ' := by
+  grind [WellTyped]
 
+@[grind →]
 theorem Program.WellTyped.unique
-    {p : Program τ n} {Δ : Context τ m} {Δ' : Context τ m'}
+    {p : Program τ} {Δ Δ' : Context τ}
     (h₁ : p.WellTypedWith Γ Δ) (h₂ : p.WellTypedWith Γ Δ') :
-      ∃ (h : m = m'), Δ = h ▸ Δ' := by
-  induction p <;> (cases h₁; cases h₂)
-  · use rfl
-  · grind
+      Δ = Δ' := by
+  induction p generalizing Γ <;> grind
+
+/-!
+## Var
+--------------------------------------------------------------------------------
+-/
+namespace Var
+
+@[simp, grind =] theorem toNat_ofNat (i : Nat) : (Var.ofNat i).toNat = i := rfl
+@[simp, grind =] theorem toNat_succ (v : Var) : v.succ.toNat = v.toNat + 1 := rfl
+
+@[simp, grind =]
+theorem inBounds_iff {v : Var} : v.InBounds Γ ↔ v.toNat < Γ.size := by rfl
+
+end Var
+
+/-!
+## Context
+--------------------------------------------------------------------------------
+-/
+namespace Context
+variable {Γ : Context τ} {v : Var}
+
+/-! ### size -/
+
+@[simp, grind =] theorem size_empty : size (∅ : Context τ) = 0 := rfl
+@[simp, grind =] theorem size_cons : size (Γ <: t) = Γ.size + 1 := rfl
+
+/-! ### getElem -/
+
+@[simp, grind =] theorem getElem_cons_zero : (Γ <: t)[Var.ofNat 0]'h = t := rfl
+@[simp, grind =] theorem getElem_cons_succ :
+    (Γ <: t)[v.succ]'h = Γ[v]'(by grind) := rfl
+
+/-! ### isUnrestricted -/
+
+@[simp, grind .] theorem isUnrestricted_empty : @isUnrestricted τ ∅ := by
+  grind [isUnrestricted]
+
+@[simp, grind =] theorem isUnrestricted_cons :
+    (Γ <: t).isUnrestricted ↔ Γ.isUnrestricted ∧ t.isUnrestricted  := by
+  unfold isUnrestricted Var.InBounds
+  constructor
+  · intro h
+    and_intros
+    · intro v
+      have := h v.succ
+      grind
+    · have := h (Var.ofNat 0)
+      grind
+  · intro h v hv
+    have : (v = Var.ofNat 0) ∨ (∃ (v' : Var), v = v'.succ) := by
+      rcases v with _|i
+      · left; rfl
+      · right; use i; rfl
+    rcases this with ⟨rfl, ⟨v, rfl⟩⟩ <;> grind
+
+end Context
